Language.v
@@ -1,0 +1,25 @@
+Require Export Coq.Strings.String.
+
+Inductive aexp : Type :=
+  | ANum : nat -> aexp
+  | AVar : string -> aexp
+  | APlus : aexp -> aexp -> aexp
+  | AMult : aexp -> aexp -> aexp.
+
+Inductive bexp : Type :=
+  | BTrue : bexp
+  | BFalse : bexp
+  | BEq : aexp -> aexp -> bexp
+  | BLe : aexp -> aexp -> bexp
+  | BNot : bexp -> bexp
+  | BAnd : bexp -> bexp -> bexp.
+
+Inductive com : Type :=
+  | CSkip : com
+  | CSeq : com -> com -> com.
+
+Bind Scope com_scope with com.
+Notation "'SKIP'" :=
+     CSkip : com_scope.
+Notation "c1 ;; c2" :=
+    (CSeq c1 c2) (at level 80, right associativity) : com_scope.
